src/Std/Data/DHashMap/Internal/Model.lean
@@ -295,6 +295,10 @@ def getₘ [BEq α] [LawfulBEq α] [Hashable α] (m : Raw₀ α β) (a : α) (h 
   (bucket m.1.buckets m.2 a).getCast a h
 
 /-- Internal implementation detail of the hash map -/
+def getEntryₘ [BEq α] [Hashable α] (m : Raw₀ α β) (a : α) (h : m.containsₘ a) : (a : α) × β a :=
+  (bucket m.1.buckets m.2 a).getEntry a h
+
+/-- Internal implementation detail of the hash map -/
 def getDₘ [BEq α] [LawfulBEq α] [Hashable α] (m : Raw₀ α β) (a : α) (fallback : β a) : β a :=
   (m.get?ₘ a).getD fallback
 
@@ -451,6 +455,9 @@ theorem get?_eq_get?ₘ [BEq α] [LawfulBEq α] [Hashable α] (m : Raw₀ α β)
 
 theorem get_eq_getₘ [BEq α] [LawfulBEq α] [Hashable α] (m : Raw₀ α β) (a : α) (h : m.contains a) :
     get m a h = getₘ m a (by exact h) := (rfl)
+
+theorem getEntry_eq_getEntryₘ [BEq α] [Hashable α] (m : Raw₀ α β) (a : α) (h : m.contains a) :
+    getEntry m a h = getEntryₘ m a (by exact h) := (rfl)
 
 theorem getD_eq_getDₘ [BEq α] [LawfulBEq α] [Hashable α] (m : Raw₀ α β) (a : α) (fallback : β a) :
     getD m a fallback = getDₘ m a fallback := by
