src/Std/Data/DHashMap/Internal/RawLemmas.lean
@@ -140,6 +140,7 @@ private meta def queryMap : Std.DHashMap Name (fun _ => Name × Array (MacroM (T
      ⟨`getKey, (``getKey_eq_getKey, #[`(getKey_of_perm _)])⟩,
      ⟨`getKeyD, (``getKeyD_eq_getKeyD, #[`(getKeyD_of_perm _)])⟩,
      ⟨`getKey!, (``getKey!_eq_getKey!, #[`(getKey!_of_perm _)])⟩,
+     ⟨`getEntry, (``getEntry_eq_getEntry, #[`(getEntry_of_perm _)])⟩,
      ⟨`toList, (``Raw.toList_eq_toListModel, #[])⟩,
      ⟨`keys, (``Raw.keys_eq_keys_toListModel, #[`(perm_keys_congr_left)])⟩,
      ⟨`Const.toList, (``Raw.Const.toList_eq_toListModel_map, #[`(perm_map_congr_left)])⟩,
@@ -375,6 +376,15 @@ theorem get_insert [LawfulBEq α] (h : m.1.WF) {k a : α} {v : β k} {h₁} :
       else
         m.get a (contains_of_contains_insert _ h h₁ (Bool.eq_false_iff.2 h₂)) := by
   simp_to_model [insert, get] using List.getValueCast_insertEntry
+
+theorem getEntry_insert [EquivBEq α] [LawfulHashable α] (h : m.1.WF) {k a : α} {v : β k} {h₁} :
+    (m.insert k v).getEntry a h₁ =
+      if h₂ : k == a then
+        ⟨k, v⟩
+      else
+        m.getEntry a (contains_of_contains_insert _ h h₁ (Bool.eq_false_iff.2 h₂)) := by
+  simp_to_model [insert, getEntry] using List.getEntry_insertEntry
+
 
 theorem get_insert_self [LawfulBEq α] (h : m.1.WF) {k : α} {v : β k} :
     (m.insert k v).get k (contains_insert_self _ h) = v := by
